lean/Main.lean
@@ -1,0 +1,4 @@
+-- This module serves as the root of the `«peregrine-lean»` library.
+-- Import modules here that should be built as part of the library.
+import Peregrine.Basic
+import Peregrine.Runtime
